# baseURI: http://www.fundontology.com/fr/FinanceLegalReference/
# imports: http://spec.edmcouncil.org/fibo/All
# imports: http://www.estrellaproject.org/lkif-core/lkif-extended
# imports: http://www.w3.org/2004/02/skos/core
# prefix: fo-fr-flr

@prefix : <http://www.fundontology.com/fr/FinanceLegalReference/> .
@prefix fibo-fnd-rel-rel: <http://www.omg.org/spec/EDMC-FIBO/FND/Relations/Relations/> .
@prefix fo-fr-flr: <http://www.fundontology.com/fr/FinanceLegalReference/> .
@prefix lkif-action: <http://www.estrellaproject.org/lkif-core/action.owl#> .
@prefix lkif-expr: <http://www.estrellaproject.org/lkif-core/expression.owl#> .
@prefix lkif-extd: <http://www.estrellaproject.org/lkif-core/lkif-extended#> .
@prefix lkif-lact: <http://www.estrellaproject.org/lkif-core/legal-action.owl#> .
@prefix lkif-leg-role: <http://www.estrellaproject.org/lkif-core/legal-role.owl#> .
@prefix lkif-lrole: <http://www.estrellaproject.org/lkif-core/legal-role.owl#> .
@prefix lkif-mereo: <http://www.estrellaproject.org/lkif-core/mereology.owl#> .
@prefix lkif-mod: <http://www.estrellaproject.org/lkif-core/time-modification.owl#> .
@prefix lkif-norm: <http://www.estrellaproject.org/lkif-core/norm.owl#> .
@prefix lkif-places: <http://www.estrellaproject.org/lkif-core/relative-places.owl#> .
@prefix lkif-proc: <http://www.estrellaproject.org/lkif-core/process.owl#> .
@prefix lkif-role: <http://www.estrellaproject.org/lkif-core/role.owl#> .
@prefix owl: <http://www.w3.org/2002/07/owl#> .
@prefix rdf: <http://www.w3.org/1999/02/22-rdf-syntax-ns#> .
@prefix rdfs: <http://www.w3.org/2000/01/rdf-schema#> .
@prefix role: <http://www.estrellaproject.org/lkif-core/role.owl#> .
@prefix skos: <http://www.w3.org/2004/02/skos/core#> .
@prefix sm: <http://www.omg.org/techprocess/ab/SpecificationMetadata/> .
@prefix untitled-ontology-148: <http://www.semanticweb.org/jziem/ontologies/2015/11/untitled-ontology-148#> .
@prefix xsd: <http://www.w3.org/2001/XMLSchema#> .

lkif-action:Agent
  owl:equivalentClass <http://spec.edmcouncil.org/fibo/FND/AgentsAndPeople/Agents/AutonomousAgent> ;
.
lkif-lrole:Social_Legal_Role
  owl:equivalentClass <http://www.omg.org/spec/EDMC-FIBO/FND/Parties/Roles/AgentInRole> ;
.
lkif-norm:Statute
  owl:equivalentClass <http://spec.edmcouncil.org/fibo/FND/Law/Jurisdiction/StatuteLaw> ;
.
<http://www.fundontology.com/Reference/ReferenceValues#ClassificationScheme_AreaOfLaw>
  lkif-mereo:component fo-fr-flr:Classification_AreaOfLaw_FinancialServices ;
  lkif-mereo:direct_part fo-fr-flr:Classification_AreaOfLaw_FinancialServices ;
  lkif-mereo:part fo-fr-flr:Classification_AreaOfLaw_FinancialServices ;
  lkif-mereo:strict_part fo-fr-flr:Classification_AreaOfLaw_FinancialServices ;
.
fo-fr-flr:
  rdf:type owl:Ontology ;
  sm:author "Jurgen Ziemer"^^xsd:string ;
  sm:copyright "Jayzed Data Models Inc."^^xsd:string ;
  rdfs:comment """Finance and Legal Reference serves 2 functions:
1) Include the external upper/core FIBO and LIKIF ontologies
2) Perform ontology alignment of FIBO and LIKF"""^^xsd:string ;
  owl:imports <http://spec.edmcouncil.org/fibo/All> ;
  owl:imports <http://www.estrellaproject.org/lkif-core/lkif-extended> ;
  owl:imports <http://www.w3.org/2004/02/skos/core> ;
  owl:versionInfo "Created with TopBraid Composer"^^xsd:string ;
.
fo-fr-flr:Classification
  rdf:type owl:Class ;
  rdfs:isDefinedBy <http://www.jayzed.com/hfr/reference/ISO_IEC_11179-2> ;
  rdfs:subClassOf <http://spec.edmcouncil.org/fibo/FND/Relations/Relations/Reference> ;
  rdfs:subClassOf [
      rdf:type owl:Restriction ;
      owl:onClass <http://spec.edmcouncil.org/fibo/FND/Arrangements/ClassificationSchemes/ClassificationScheme> ;
      owl:onProperty lkif-mereo:component_of ;
      owl:qualifiedCardinality "1"^^xsd:nonNegativeInteger ;
    ] ;
  skos:definition "An Item in a Classification Scheme."^^xsd:string ;
.
fo-fr-flr:ClassificationScheme_AreaOfLaw
  rdf:type fo-fr-flr:LegalClassificationScheme ;
  rdfs:label "Areas of Law"^^xsd:string ;
.
fo-fr-flr:Classification_AreaOfLaw_FinancialServices
  rdf:type fo-fr-flr:LegalClassification ;
  lkif-mereo:component_of <http://www.fundontology.com/Reference/ReferenceValues#ClassificationScheme_AreaOfLaw> ;
  lkif-mereo:direct_part_of <http://www.fundontology.com/Reference/ReferenceValues#ClassificationScheme_AreaOfLaw> ;
  lkif-mereo:part_of <http://www.fundontology.com/Reference/ReferenceValues#ClassificationScheme_AreaOfLaw> ;
  lkif-mereo:strict_part_of <http://www.fundontology.com/Reference/ReferenceValues#ClassificationScheme_AreaOfLaw> ;
  rdfs:label "Financial Services area of law"^^xsd:string ;
.
fo-fr-flr:ExecutiveBody
  rdf:type owl:Class ;
  rdfs:comment "The executive branch is the body of the government that has its authority and responsibility for the daily administration of the state. The executive branch executes, or enforces the law. "^^xsd:string ;
  rdfs:isDefinedBy <https://en.wikipedia.org/wiki/Executive_(government)> ;
  rdfs:label "Executive Branch"^^xsd:string ;
  rdfs:label "Legislative Body"^^xsd:string ;
  rdfs:subClassOf lkif-lact:Public_Body ;
  owl:disjointWith lkif-lact:Legislative_Body ;
.
fo-fr-flr:FinanceStatute
  rdf:type owl:Class ;
  rdfs:label "Finance Statute"^^xsd:string ;
  rdfs:subClassOf <http://spec.edmcouncil.org/fibo/FND/Law/Jurisdiction/StatuteLaw> ;
  owl:equivalentClass [
      rdf:type owl:Class ;
      owl:intersectionOf (
          [
            rdf:type owl:Restriction ;
            owl:hasValue fo-fr-flr:Classification_AreaOfLaw_FinancialServices ;
            owl:onProperty <http://spec.edmcouncil.org/fibo/FND/Relations/Relations/isClassifiedBy> ;
          ]
          <http://spec.edmcouncil.org/fibo/FND/Law/Jurisdiction/StatuteLaw>
        ) ;
    ] ;
  skos:definition "A Statute Law pertaining to Financial Industry."^^xsd:string ;
.
fo-fr-flr:FinancialJusrisdiction
  rdf:type owl:Class ;
  rdfs:label "Financial Jurisdiction"^^xsd:string ;
  rdfs:subClassOf <http://spec.edmcouncil.org/fibo/FND/Law/Jurisdiction/Jurisdiction> ;
.
fo-fr-flr:FinancialRegulation
  rdf:type owl:Class ;
  rdfs:isDefinedBy <https://en.wikipedia.org/wiki/Financial_regulation> ;
  rdfs:label "Financial Regulation"^^xsd:string ;
  rdfs:subClassOf lkif-norm:Regulation ;
  skos:definition "Financial regulation is a form of regulation or supervision, which subjects financial institutions to certain requirements, restrictions and guidelines, aiming to maintain the integrity of the financial system. This may be handled by either a government or non-government organization. Financial regulation has also influenced the structure of banking sectors, by decreasing borrowing costs and increasing the variety of financial products available."^^xsd:string ;
.
fo-fr-flr:LegalClassification
  rdf:type owl:Class ;
  rdfs:label "Legal Classification"^^xsd:string ;
  rdfs:subClassOf fo-fr-flr:Classification ;
  rdfs:subClassOf [
      rdf:type owl:Restriction ;
      owl:onClass fo-fr-flr:LegalClassificationScheme ;
      owl:onProperty lkif-mereo:component_of ;
      owl:qualifiedCardinality "1"^^xsd:nonNegativeInteger ;
    ] ;
.
fo-fr-flr:LegalClassificationScheme
  rdf:type owl:Class ;
  rdfs:label "Legal Classification Scheme"^^xsd:string ;
  rdfs:subClassOf <http://spec.edmcouncil.org/fibo/FND/Arrangements/ClassificationSchemes/ClassificationScheme> ;
  owl:equivalentClass <http://spec.edmcouncil.org/fibo/FBC/FunctionalEntities/RegulatoryAgencies/Regulation> ;
.
fo-fr-flr:RegulatoryAuthority
  rdf:type owl:Class ;
  rdfs:isDefinedBy <https://en.wikipedia.org/wiki/Regulatory_agency> ;
  rdfs:label "Regulatory Authority"^^xsd:string ;
  rdfs:subClassOf fo-fr-flr:ExecutiveBody ;
  owl:equivalentClass <http://spec.edmcouncil.org/fibo/FBC/FunctionalEntities/RegulatoryAgencies/RegulatoryAgency> ;
  skos:definition "A regulatory agency (also regulatory authority, regulatory body or regulator) is a public authority or government agency responsible for exercising autonomous authority over some area of human activity in a regulatory or supervisory capacity. An independent regulatory agency is a regulatory agency that is independent from other branches or arms of the government."^^xsd:string ;
.
fo-fr-flr:RegulatoryAuthority_SecuritiesAndExchangeCommission
  rdf:type fo-fr-flr:RegulatoryAuthority ;
  rdfs:label "U.S. Securities and Exchange Commission"^^xsd:string ;
  owl:sameAs <http://spec.edmcouncil.org/fibo/FBC/FunctionalEntities/USJurisdiction/USRegulatoryAgencies/SecuritiesAndExchangeCommission> ;
.
fo-fr-flr:Rulemaking
  rdf:type owl:Class ;
  rdfs:isDefinedBy <https://en.wikipedia.org/wiki/Rulemaking> ;
  rdfs:label "Rulemaking"^^xsd:string ;
  rdfs:subClassOf lkif-lact:Public_Act ;
  skos:definition "In administrative law, rule-making is the process that executive and independent agencies use to create, or promulgate, regulations. In general, legislatures first set broad policy mandates by passing statutes, then agencies create more detailed regulations through rulemaking."^^xsd:string ;
.
